#set math.equation(numbering: "(1)")
#set text(
font: "Palatino Linotype",size: 11pt)
#set page(margin: (x: 1cm, y: 1cm), numbering: "1/1")
#import "@preview/physica:0.9.6": *
#place(top + right, rect(inset: 3pt)[MATH 541 HW 7 Harry Luo
])
= 1
#align(
  left,
  rect(inset: 8pt)[#image("assets/2025-10-28-16-12-27.png")]
)
We lable BINGE as $(1 2 3 4 5)$ and BEGIN as $( 1 5 4 2 3)$. We see that the permulation that sends BINGE to BEGIN is $ 
sigma = display(mat(1, 2,3,4,5; 1,5,4,2,3)) = (2 med 5med 3med 4)  
$ 
 We count the inversions: $(4,5), (2,5), (3,5), (2,4), (3,4).$  So $#rect(inset: 8pt)[
$ display( "inv"(sigma) = 5.)$
]
$ 

 Now, we take $sigma'$ as BEING to BINGE, and $sigma''$ as BEING to BEGIN. We notice that $ 
 sigma '' = sigma compose sigma' \ => "inv"(sigma'') = "inv"(sigma) + "inv"(sigma') = 5 + "inv"(sigma') = "inv"(sigma')+1 mod 2
 $ 
So it's obvious that $sigma'$ and $sigma''$ have different parities.

To verify, consider $ 
sigma' = display(mat(1,2,3,4,5; 1,3,4,5,2))   
$ 
inversions of $sigma'$ are $(2,3), (2,4), (2,5).$ So $"inv"(sigma') = 3,$ which is odd. 

Consider $ 
sigma'' = display(mat(1,2,3,4,5; 1,2,5,3,4))  
$ 
The inversions are $(3,5), (4,5).$ So $"inv"(sigma'') = 2,$ which is even -- different parity from $sigma'.$

#pagebreak()
= 2 
#align(
  left,
  rect(inset: 8pt)[#image("assets/2025-10-28-16-28-01.png")]
)

== a. 
Recall that $S_n = angle.l (i j) angle.r $, where $1 <= i <= j <= n$. For each such pair of $i, j$ transposition, we  can write $ 
( i med  j) = (1 med i) (1 med j) (1med i).
$ 
In other words, each of the generator of $S_n$ can be written in terms of generators ${(1 med k)| 2<= k <= n} $ where the size of this new generating set is $n-1.$ Therefore , $S_n$ can be generated by $n-1$ transpositions $(1 med i), (2<= i <= n)$.

== b.
Define an adjacent transposition $t_i := (i med i+1)$ . 
We show that for $1<= i <= n-1, med j = i+k:$ $ 
(i med j) &= (i med i+1) (i+1 med i+2) dots (j-1 med j) (j-2 med j-1) dots (i med i+1) \ 
& = t_i med t_(i+1) dots med t_(j-1)med t_(j-2) dots med t_i
$ 
so that each $(i med j)$ can be decomposed into a product of adjacent transpositions. Since the set ${(i med j) | 1<= i < j <= n} $ generates $S_n,$ the set of adjacent transpositions ${(i med i+1) | 1<= i <= n-1} $ also generates $S_n.$

== c
Consider the transposition of two adjacent elements $( k med k+1)$ (where $k$ is arbitrary). This can be expressed in terms of the transposition $(1 med 2)$ and the long cycle $rho := (1 med 2 med dots n)$ as follows: $ 
(k med k+1) = rho^(k-1) med (1 med 2) med rho^(-(k-1)) 
$ 
Concretely, we can follow the mapping: $rho^(-(k-1)):k -> 1, quad (1 med 2):1 -> 2, quad rho^(k-1):2 ->  k+1$.

By varing $k,$ we see that $angle.l(1 med 2), med rho angle.r$  generates all adjacent transpositions, which in turn generates $S_n.$ 

== d.
From (a), we know that $S_n = angle.l (1 2) med (1 3) dots (1 n) angle.r $. Since $A_n = {pi in S_n, pi "is even permutation"}$ , $pi$ can be written as products even number of transpositions , i.e. $product_k (1 k)$.  This can be grouped into pairs of $ 
(1 i ) (1 j) = (1 i j) quad (2 <= i < j <= n)
$ 
which is exactly the set of 3-cycles that we want. Therefore, $A_n$ is generated by the set of 3-cycles of the form $ 
(1 i j) , quad 2 <= i < j <= n.
$

== e.
By part d, we know that for any $sigma in A_n, med sigma = product tau_i$, where each $tau_i$ is a 3-cycle $(1 i j)$. We know that $tau^3 = 1.$   

Then for any $g in h(A_n), g = h(sigma)$. Homomorphism gives $ 
g = h(sigma) = h(product tau_i) = product h(tau_i) 
$ 
and abelianity gives $ 
g^3 = (h(sigma))^3 = product (h(tau_i))^3 = product h(tau_i^3) = product h(1) = 1.
$ 




#pagebreak()
= 3
#align(
  left,
  rect(inset: 8pt)[#image("assets/2025-10-28-21-30-38.png")]
)
Construct a mapping (with $n >= 3$ ) $phi: S_(n-2)-> A_n$ as $ 
phi(sigma) = cases(sigma quad & sigma " even", sigma (n med n-1) quad quad  &sigma "odd",) 
$ where $sigma in S_(n-2)$, and it permutes the first $n-2$ elements, and leaves $n-1$ and $n$ fixed.

We will show that $phi$ is an injective homomorphism, and use the first isomorphism theorem to conclude that $S_(n-2) tilde.equiv Im(phi) subset A_n. $  
 
First, $Im(phi) subset A_n$. Since for any $sigma in S_(n-2)$, if :
- $sigma$ even, then $phi(sigma) = sigma in A_n.$
- $sigma$ odd, then $phi(sigma) = sigma (n med n-1).$ Note that $(n med n-1)$ is also odd, so the product of two odd permutations is even, and thus $phi(sigma) in A_n.$

Second, $phi(sigma tau) = phi(sigma) phi(tau)$ for any $sigma, tau in S_(n-2)$. Indeed: 
- If $sigma, tau$ have the same parity, then $sigma tau$ is even, and so $ 
phi(sigma tau) = sigma tau = phi(sigma) phi(tau) ,
$ where the last equality holds because in the case both $sigma, tau$ are odd, $phi(sigma) phi(tau) = sigma (n med n-1) tau (n med n-1)= sigma tau$, since $sigma, tau$ commute with $(n med n-1)$ as they only permute the first $n-2$ elements.
- If $sigma, tau$ have different parities, then $sigma tau$ is odd, and so $ 
phi(sigma tau) = sigma tau (n med n-1)= phi(sigma) phi(tau) .
$ 
   
Finally, we show that $ker(phi) = {e}.$ Consider $phi(sigma) = e.$ If: 
- $sigma$ even, then $phi(sigma) = sigma = e,$ so $sigma = e.$
- $sigma$ odd, then $phi(sigma) = sigma (n med n-1) = e,$ so $sigma = (n med n-1),$ which is a contradiction since $sigma in S_(n-2)$ only permutes the first $n-2$ elements so $sigma eq.not (n med n-1)$.

Collectively, we have shown that $phi$ is an injective homomorphism, so by the first isomorphism theorem, $ S_(n-2) tilde.equiv Im(phi) subset A_n. $     
In other words, $A_n$ contains a subgroup isomorphic to $S_(n-2)$ for $n >= 3.$ 


#pagebreak()
= 4
#align(
  left,
  rect(inset: 8pt)[#image("assets/2025-10-30-15-29-31.png")]
)
== a 
We show that $G_(g a) subset g G_a g^(-1), $ and then $g G_a g^(-1) subset G_(g a)$.  
1. For any $h in G_(g a),$ we have by the definition of stablizer that $ 
h(g a) = g a => g^(-1) h g a = a => g^(-1) h g in G_a 
$ and so $ h in G_a.$ 
Therefore, $G_(g a) subset g G_a g^(-1).$
2. For any $h in g G_a g^(-1), $ and for any $k in G_a,$  we have $
   h = g k g^(-1)  => h g a = g k g^(-1) g a = g k a = g a
$ and so $h in G_(g a).$
Therefore, $g G_a g^(-1) subset G_(g a).$ Collectively, we have $G_(g a) = g G_a g^(-1).$

== b
We know that the kernel is the intersection of all stabilizers:
$
ker = {k in G | k x = x forall x in A} = inter.big_(x in A) G_x
$ 
Since the action is transitive, the orbit of any $x in A$ is the whole set $A,$ i.e. $ 
cal(O)_a = A 
$ and so for any $x in A,$ there exists $g in G$ such that $x = g a.$ Therefore,$ 
ker = inter.big_(x in A) G_x=inter.big_(g in G) G_(g a)
$ 
by part a, we have $
ker = inter.big_(g in G) g G_a g^(-1).
$


== c
Given $G <= S_A$ and G is transitive, then $ 
ker = {g in G| g s = s , forall s in A}  = {e} 
$ since each $g in G$ is a permutation on $A,$ and the only permutation that fixes all elements is the identity permutation.  

By part b, a transitive action has kernel equal to the intersection of all conjugates of a stabilizer. Therefore, $ 
 {e}=ker = inter.big_(g in G) g G_a g^(-1).
$ 


== d
Given that $G$ is abelian in addition to being a transitive subgroup of $S_A,$ we have $ 
g G_a g^(-1)= G_a,  
$ since for any $h in G_a,$ $g h g^(-1) = h g g^(-1) = h in G_a.$ Therefore by part c, $ 
inter.big_(g in G_a) g G_a g^(-1) = inter.big_(g in G) G_a = G_a = {e}.
$ Thus the set $G - {e} = G - G_a$, and so for any $g in G - {e}, a in A: med g in.not G_a,$ i.e. $ g a = g(a) eq.not a. $       

Further, by Orbit-stabilizer theorem, $ 
|G| = |O_a| dot |G_a|, 
$ but since $G_a = {e}, med |G_a| = 1,$ and since the action is transitive, $|O_a| = |A|.$ Therefore, $ 
|G| = |A|. 
$


#pagebreak()
= 5
#align(
  left,
  rect(inset: 8pt)[#image("assets/2025-10-31-20-31-59.png")]
)

== a 
It's helpful to first writeout the elements of $S_3 = {e , (1 med 2), (1 med 3), (2 med 3), (1 med 2 med 3), (1 med 3 med 2)}.$ 

For any $sigma in S_3, $ the action is that $sigma (i, j) = ( sigma(i), sigma(j)).$
Notice that for $i eq.not j,$ $sigma(i) eq.not sigma(j)$ and for $i = j,$ $sigma(i) = sigma(j)$. So the action preserves the property of being a distinct or identical pair. Therefore, the action partitions $Omega$ into two orbits $ 
cal(O_1) = {(1,1),(2,2),(3,3)}; \ 
cal(O_2) = {(i,j)| i eq.not j}, quad |cal(O_2)|=6
 
$ 



== b 
We first write this action into permutation representation. Labling elements of $Omega$ as $ 1: (1,1), 2:(1,2), 3:(1,3),\ 4:(2,1), 5:(2,2), 6:(2,3), \ 7:(3,1), 8:(3,2), 9:(3,3) $ We can find the permutation representation of each element in $S_3$, and from which we can find the cycle decomposition:
$ 
e: e \ 
(1 2): display(mat(1,2,3,4,5,6,7,8,9;5,4,6,2,1,3,8,7,9)) = (1 5)(2 4)(3 6)(7 8)(9)   ,\ 
(1 3): display(mat(1,2,3,4,5,6,7,8,9; 5,4,6,2,1,3,8,7,9)) = (1 9) (2 8)(3 7)(4 6)(5), \ 
(2 3): display(mat(1,2,3,4,5,6,7,8,9; 1,3,2,7,9,8,4,6,5)) = (1) (2 3) (4 7) (5 9) (6 8), \ 
(1 2 3): display(mat(1,2,3,4,5,6,7,8,9; 5,6,4,8,9,7,2,3,1))= (1 5 9)(2 6 7)(3 4 8) ,\ 
(1 3 2): display(mat(1,2,3,4,5,6,7,8,9; 9,7,8,3,1,2,6,4,5))  = (1 9 5)(2 7 6)(3 8 4)
$ 



== c 
1. For orbit $cal(O_1)$, we pick $a = (1,1).$
Stabilizer by definition is $ 
G_(S_3) = {sigma in S_3 | sigma (1,1) = (1,1)} . 
$ 
since $sigma(1) = 1, sigma = e "or" (2 3)$ , and so $ 
G_(S_3) = {e, (2 med 3)} .
$ 




2. For orbit $cal(O_2)$, we pick $b = (1,2).$
Pick $b = (1,2)$. 
Stabilizer by definition is $
G_(S_3) = {sigma in S_3 | sigma (1,2) = (1,2)} .
$
Since $sigma(1) = 1, sigma(2) = 2, sigma = e$ , and so $
G_(S_3) = {e} .
$ 





